\subsection{Exercises}
\subsubsection{1.}
Compute $\sqrt{i}$, let us observe
\begin{align*}
(x + iy)^2 &= 0 + i \\
x^2 + 2xiy - y^2 = 0 + i
\end{align*}
Which give us the following system:
\begin{align*}
x^2 - y^2 = 0 \\
2xy = 1
\end{align*}
So that 
\begin{align*}
(x^2 + y^2)^2 &= (x^2 - y^2)^2 + 4x^2y^2 \\
&= 1 \\
\end{align*}
so that we have
\begin{align*}
	x^2 &= \frac{1}{2} \\
	y^2 &= \frac{1}{2}
\end{align*}
so that we must set up the possible values of $x$ and $y$ so that $ \beta $ has the right sign.
\begin{align*}
z_1 &= \frac{1}{\sqrt{2}} + i\frac{1}{\sqrt{2}} \\
z_2 &= -\frac{1}{\sqrt{2}} - i\frac{1}{\sqrt{2}}
\end{align*}
\rule{\textwidth}{1pt}
Let us find $x,y$ so that:
\begin{align*}
(x + iy)^2 &= -i \\
x^2 + 2xiy - y^2 = -i
\end{align*}
so that
\begin{align*}
x^2 - y^2 &= -i \\
2xy &= -1 \\
x^2 + y^2 &= 1  
\end{align*}
and we get:
\begin{align*}
x^2 = \frac{1}{2} \\
y^2 = \frac{1}{2}
\end{align*}
and since we need $2xy = -1$, we see that the roots are:
\begin{align*}
z_1 &= \frac{1}{\sqrt{2}} - \frac{1}{\sqrt{2}}i \\
z_2 &= -\frac{1}{\sqrt{2}} + \frac{1}{\sqrt{2}}i
\end{align*}
\rule{\textwidth}{1pt}
\begin{align*}
(x + iy)^2 &= 1 + i \\
x^2 + 2xiy - y^2 &= 1 + i\\
\end{align*}
and we get the system of equalities:
\begin{align*}
x^2 - y^2 = 1 \\ 
2xy = 1
\end{align*}
and after some algebra:
\begin{align*}
x^2 &= \frac{\sqrt{2} + 1}{2} \\
y^2 &= \frac{-1 + \sqrt{2} }{2}
\end{align*}
and having the condition of $x \cdot y > 0 $, we conclude:
\begin{align*}
z_1 &= \sqrt{\frac{\sqrt{2} + 1}{2}} + i \sqrt{\frac{-1 + \sqrt{2}}{2} }\\
z_2 &= -\sqrt{\frac{(\sqrt{2} + 1)}{2}} - i \sqrt{ \frac{-1 + \sqrt{2} }{2} }
\end{align*}
\rule{\textwidth}{1pt}
We want to find $x,y$ so that:
\begin{align*}
(x + iy)^2 = \frac{1 - i \sqrt{3}}{2}
\end{align*}
which give us the system of equalities
\begin{align*}
\begin{cases}
x^2 - y^2 &= \frac{1}{2} \\
2xy &= -\frac{\sqrt{3}}{2} 
\end{cases}
\end{align*}
which ends up with the specification of: 
\begin{align*}
	x^2 &= \frac{3}{4} \\
	y^2 &= \frac{1}{4}
\end{align*}
So that we found:
\begin{align*}
z_1 &= \frac{\sqrt{3}}{2} - i\frac{1}{2} \\
z_2 &= -\frac{\sqrt{3}}{2} + i \frac{1}{2}
\end{align*}
\subsubsection{2.} Find the four values of $ \sqrt[4]{-1} $

We begin then with looking solutions of the form:
\begin{align*}
(x + iy)^4	==ssds
\end{align*} 
